\section{For a cpo $D$, consider the function $Apply: [D \rightarrow D] \times D \rightarrow D$ for which $Apply (f, x) = f(x)$. Prove that $Apply$ is continuous.}

As established in class, $[D \rightarrow D]$  denotes a ccpo of continuous functions. \\
Let $F$ a be a subset of $[D \rightarrow D]$ such that it is a chain. Let furthermore $C$ be a subset of $D$ such that it is a chain. Since $F$ is a set of \underline{continuous} functions, it must be true that
\begin{align}
	& ( \sqcup ( f \text{ } C ) = f \text{ } \sqcup C ) \text{ } | \text{ } \forall f \in F \label{eq:cont:given:x}
\end{align}
When comparing function spaces such as $F$ it is for all $f_i,f_{i+1} \in F$ that
\begin{align}
	& f_i \leq f_{i+1} \text{ if } f_i \text{ } x \leq f_{i+1} \text{ } x \text{ } \text{ } | \text{ } \forall x \in D
\end{align}
Since $F$ is a \underline{ccpo} of functions, it must be that
\begin{align}
						& \exists \sqcup F \text{ such that } ( f \leq \sqcup F ) \text{ } | \text{ } \forall f \in F \\
\Rightarrow & (( f \text{ } x \leq \sqcup F \text{ } x ) \text{ } | \text{ } \forall f \in F ) \text{ } | \text{ } \forall x \in D \\
\Rightarrow	& ( \sqcup \{ f \text{ } x \text{ } | \text{ } \forall f \in F \} = ( \sqcup F ) \text{ } x ) \text{ } | \text{ } \forall x \in D \\
\Rightarrow	& ( \sqcup \{ F \text{ } x \} = (\sqcup F) \text{ } x ) \text{ } | \text{ } \forall x \in C \label{eq:cont:given:f}
\end{align}
In order for $Apply$ to be continuous, it must be that for all $f \in F$ and $x \in C$
\begin{align}
	& \sqcup Apply \text{ } (f,x) = Apply \text{ } \sqcup (f,x)
\end{align}
It is given that a function is continuous if it is continuous in each of its parameters. Therefore, if $Apply$ is continuous in its parameters, it must be continuous itself as well. By fixing single parameters, partially applied functions can be constructed that have the same properties (such as the continuity) for the remaining parameters as $Apply$. Consequently, by fixing $f$, the partially applied function $Apply_f$ can be constructed, that allows the evaluation of the continuity of $Apply$ in $x$. Respectively, $Apply_x$ allows the evaluation of the continuity of $Apply$ in $f$ by fixing $x$. If both $Apply_f$ and $Apply_x$ are contiuous, $Apply$ must be continuous, too. Now in order for $Apply_f$ and $Apply_x$ to be continuous, it must be true that
\begin{align}
	& ( \sqcup ( Apply_f \text{ } C ) = Apply_f \text{ } \sqcup C ) \text{ } | \text{ } \forall f \in F \label{eq:cont:req:x} \\
	& ( \sqcup ( Apply_x \text{ } F ) = Apply_x \text{ } \sqcup F ) \text{ } | \text{ } \forall x \in C \label{eq:cont:req:f}
\end{align}
Since $Apply \text{ } (f,x) = f \text{ } x$, any $Apply_f \text{ } x$ can also be expressed as $f \text{ } x$. Thus, equation \ref{eq:cont:req:x} results to
\begin{align}
	& ( \sqcup ( f \text{ } C ) = f \text{ } \sqcup C \text{ } ) | \text{ } \forall f \in F
\end{align}
which is provided by equation \ref{eq:cont:given:x}. Consequently it is that $Apply_f$ is continuous, implying that	\textbf{$Apply$ is continuous in $x$}. 
Furthermore, $Apply \text{ } (f,x) = f \text{ } x$ requires that equation \ref{eq:cont:req:f} results to
\begin{align}
	& ( \sqcup ( F \text{ } x ) = (\sqcup F) \text{ } x ) \text{ } | \text{ } \forall x \in D
\end{align}
which is provided to equation \ref{eq:cont:given:f}. Consequently it is that $Apply_x$ is continuous, implying that	\textbf{$Apply$ is continuous in $f$}. 
Thus it is proven that $Apply$ is continuous both in $f$ and in $x$, Subsequentially, it must be true that \textbf{$Apply$ is continuous}.